cleanup: make PrivateKeys more aware of PKI

src/lib/state/DY.Lib.State.PKI.fst
@@ -25,8 +25,8 @@ open DY.Lib.State.Map
 
 [@@ with_bytes bytes]
 type public_key_type =
-  | PkEnc: [@@@ with_parser #bytes ps_string] usage:string -> public_key_type
-  | Verify: [@@@ with_parser #bytes ps_string] usage:string -> public_key_type
+  | LongTermPkEncKey: [@@@ with_parser #bytes ps_string] usage:string -> public_key_type
+  | LongTermSigKey: [@@@ with_parser #bytes ps_string] usage:string -> public_key_type
 
 %splice [ps_public_key_type] (gen_parser (`public_key_type))
 %splice [ps_public_key_type_is_well_formed] (gen_is_well_formed_lemma (`public_key_type))
@@ -54,16 +54,24 @@ instance map_types_pki: map_types pki_key pki_value = {
   ps_value_t = ps_pki_value;
 }
 
+val public_key_type_to_usage:
+  public_key_type ->
+  usage
+let public_key_type_to_usage sk_type =
+  match sk_type with
+  | LongTermPkEncKey usg -> PkKey usg empty
+  | LongTermSigKey usg -> SigKey usg empty
+
 val is_public_key_for:
   {|crypto_invariants|} -> trace ->
   bytes -> public_key_type -> principal -> prop
 let is_public_key_for #cinvs tr pk pk_type who =
   match pk_type with
-  | PkEnc usg -> (
-    is_encryption_key (PkKey usg empty) (principal_label who) tr pk
+  | LongTermPkEncKey usg -> (
+    is_encryption_key (public_key_type_to_usage pk_type) (principal_label who) tr pk
   )
-  | Verify usg -> (
-    is_verification_key (SigKey usg empty) (principal_label who) tr pk
+  | LongTermSigKey usg -> (
+    is_verification_key (public_key_type_to_usage pk_type) (principal_label who) tr pk
   )
 
 // The `#_` at the end is a workaround for FStarLang/FStar#3286
