examples/iso_dh/DY.Example.DH.Protocol.Total.Proof.fst
@@ -130,7 +130,7 @@ val compute_message2_proof:
     event_triggered tr bob (Respond1 alice bob gx (dh_pk y) y) /\
     is_publishable tr gx /\
     bytes_invariant tr y /\
-    is_signature_key (SigKey "DH.SigningKey" empty) (principal_label bob) tr sk_b /\
+    is_private_key_for tr sk_b (LongTermSigKey "DH.SigningKey") bob /\
     is_secret (principal_label bob) tr n_sig /\
     SigNonce? (get_usage n_sig)
   )
@@ -175,7 +175,7 @@ val decode_and_verify_message2_proof:
   (requires
     is_publishable tr msg2_bytes /\
     is_secret (principal_state_label alice alice_si) tr x /\
-    is_verification_key (SigKey "DH.SigningKey" empty) (principal_label bob) tr pk_b
+    is_public_key_for tr pk_b (LongTermSigKey "DH.SigningKey") bob
   )
   (ensures (
     match decode_and_verify_message2 msg2_bytes alice x pk_b with
@@ -218,7 +218,7 @@ val compute_message3_proof:
     event_triggered tr alice (Initiate2 alice bob (dh_pk x) gy (dh x gy)) /\
     is_publishable tr gx /\ is_publishable tr gy /\
     gx = dh_pk x /\
-    is_signature_key (SigKey "DH.SigningKey" empty) (principal_label alice) tr sk_a /\
+    is_private_key_for tr sk_a (LongTermSigKey "DH.SigningKey") alice /\
     is_secret (principal_label alice) tr n_sig /\
     SigNonce? (get_usage n_sig)
   )
@@ -259,7 +259,7 @@ val decode_and_verify_message3_proof:
     is_publishable tr msg3_bytes /\
     is_publishable tr gx /\
     is_secret (principal_state_label bob bob_si) tr y /\
-    is_verification_key (SigKey "DH.SigningKey" empty) (principal_label alice) tr pk_a
+    is_public_key_for tr pk_a (LongTermSigKey "DH.SigningKey") alice
   )
   (ensures (
     let gy = dh_pk y in
